modules/HMod.v
@@ -11,75 +11,83 @@ Require Export HMod2Mod.
 
 Set Implicit Arguments.
 
-Definition fnsems_keys {T} (fn: gname) (fnsems: alist gname ((list string) * T)) :=
-  match (alist_find fn fnsems) with
-  | Some (keys, body) => keys
-  | None => []
-  end.
+  (* TODO: move to a right place *)
+  Lemma unfold_iter_eq (E : Type -> Type) (A B : Type) (f : A -> itree E (A + B)) (x : A)
+    :
+    ITree.iter f x = lr <- f x;;
+                     match lr with
+                     | inl l => tau;; ITree.iter f l
+                     | inr r => Ret r
+                     end.
+  Proof.
+    eapply bisim_is_eq. eapply unfold_iter.
+  Qed.
 
 Module HModSem.
 Section HMODSEM.
   Context `{Σ: GRA.t}.
 
   Record t: Type := mk {
+    scopes : list string;
     fnsems : alist gname (list string * (Any.t -> itree hmodE Any.t));
-    initial_st : alist string Any.t;
+    initial_st : alist key Any.t;
     initial_cond: iProp;
-    well_scoped:
-      forall fn, incl (fnsems_keys fn fnsems) (List.map fst initial_st);
+    well_scoped_fns:
+      forall fn, incl (fnsems_scopes fn fnsems) scopes;
+    well_scoped_init:
+      incl (List.map (fst ∘ fst) initial_st) scopes;
   }.
 
   Record wf (ms: t): Prop := mk_wf {
-    wf_fns: List.NoDup (List.map fst ms.(fnsems));                                 
-    wf_keys: List.NoDup (List.map fst ms.(initial_st));
+    wf_fns: List.NoDup (List.map fst ms.(fnsems));
+    wf_scopes: List.NoDup ms.(scopes);
   }.
 
   (**** Linking ****)
 
   Program Definition add ms1 ms2: t := {|
     fnsems := ms1.(fnsems) ++ ms2.(fnsems);
+    scopes := ms1.(scopes) ++ ms2.(scopes);
     initial_st := ms1.(initial_st) ++ ms2.(initial_st);
     initial_cond := (initial_cond ms1) ∗ (initial_cond ms2);
   |}.
   Next Obligation.
-    ii. unfold fnsems_keys in H. des_ifs. 
+    ii. unfold fnsems_scopes in H. des_ifs. 
     rewrite alist_find_app_o in Heq. des_ifs.
     {
-      hexploit (ms1.(well_scoped) fn a). 
-      { unfold fnsems_keys. des_ifs. }
-      i. rewrite List.map_app. eapply in_or_app. eauto.
+      hexploit (ms1.(well_scoped_fns) fn a). 
+      { unfold fnsems_scopes. des_ifs. }
+      i. eapply in_or_app. eauto.
     }
     {
-      hexploit (ms2.(well_scoped) fn a). 
-      { unfold fnsems_keys. des_ifs. }
-      i. rewrite List.map_app. eapply in_or_app. eauto.
+      hexploit (ms2.(well_scoped_fns) fn a). 
+      { unfold fnsems_scopes. des_ifs. }
+      i. eapply in_or_app. eauto.
     }
+  Qed.
+  Next Obligation.
+    ii. destruct ms1, ms2. ss.
+    rewrite map_app in H. apply in_or_app. apply in_app_or in H.
+    destruct H; eauto.
   Qed.
 
   (**** Wrapper ****)
 
-  Definition wrap keys : forall T, hmodE T -> hmodE T :=
+  Definition wrap scopes : forall T, hmodE T -> hmodE T :=
     (fun T e =>
        match e with
-       | inr1 (inr1 (inl1 (SPut k v))) =>
-           if existsb (eqb k) keys then e else inr1 (inr1 (inr1 (Choose T)))
-       | inr1 (inr1 (inl1 (SGet k))) =>
-           if existsb (eqb k) keys then e else inr1 (inr1 (inr1 (Choose T)))
+       | inr1 (inr1 (inl1 (SPut (s,f) v))) =>
+           if existsb (eqb s) scopes then e else inr1 (inr1 (inr1 (Choose T)))
+       | inr1 (inr1 (inl1 (SGet (s,f)))) =>
+           if existsb (eqb s) scopes then e else inr1 (inr1 (inr1 (Choose T)))
        | _ => e
        end).
 
   Definition wrap_body (kb: list string * (Any.t -> itree hmodE Any.t)) :=
     fun arg => translate (wrap kb.1) (kb.2 arg).
   
-  Definition wrap_pgE keys : pgE ~> itree hmodE :=
-    (fun _ e =>
-       match e with
-       | SPut k v => if existsb (eqb k) keys then trigger (SPut k v) else (Ret tt↑)
-       | SGet k => if existsb (eqb k) keys then trigger (SGet k) else (Ret tt↑)
-       end).
-
   Definition to_mod (ms: t) (r: Σ): ModSem.t := {|
-    ModSem.fnsems := List.map (fun '(fn, kb) => (fn, interp_hp_fun (wrap_body kb))) ms.(fnsems);
+    ModSem.fnsems := List.map (map_snd (interp_hp_fun ∘ wrap_body)) ms.(fnsems);
     ModSem.initial_st := Any.pair (alist_encode ms.(initial_st)) r↑;
   |}.
 
@@ -108,69 +116,39 @@ Section HMOD.
 End HMOD.
 End HMod.
 
-Section HModProd.
-  Context `{Σ: GRA.t}.
-
-  Lemma unfold_iter_eq (E : Type -> Type) (A B : Type) (f : A -> itree E (A + B)) (x : A)
-    :
-    ITree.iter f x = lr <- f x;;
-                     match lr with
-                     | inl l => tau;; ITree.iter f l
-                     | inr r => Ret r
-                     end.
-  Proof.
-    eapply bisim_is_eq. eapply unfold_iter.
-  Qed.
-
-  Lemma combine_quant A (B: A -> Type) (P: forall a (b: B a), Prop)
-      (PR: forall (ab: sigT B), P (projT1 ab) (projT2 ab)):
-    forall a b, P a b.
-  Proof. i. eapply (PR (existT a b)). Qed.
-
-  Definition IstEq keys: alist string Any.t -> alist string Any.t -> iProp :=
-    fun st_src st_tgt => ⌜st_src = st_tgt ∧ incl keys (List.map fst st_src)⌝%I.
-
-  Definition IstProd (IstL IstR : alist string Any.t -> alist string Any.t -> iProp) : alist string Any.t -> alist string Any.t -> iProp :=
-    fun st_src st_tgt => (∃ st_srcL st_tgtL st_srcR st_tgtR,
-      ⌜st_src = st_srcL ++ st_srcR /\ st_tgt = st_tgtL ++ st_tgtR⌝ ∗
-      IstL st_srcL st_tgtL ∗ IstR st_srcR st_tgtR)%I.
-
-End HModProd.
-
-
 Module HModWrap.
 Section RED.
   Context `{Σ: GRA.t}.
 
   Lemma transl_bind
     A B
-    keys
+    scopes
     (itr: itree hmodE A) (ktr: A -> itree hmodE B)
     :
-    translate (HModSem.wrap keys) (itr >>= ktr) = a <- (translate (HModSem.wrap keys) itr);; (translate (HModSem.wrap keys) (ktr a))
+    translate (HModSem.wrap scopes) (itr >>= ktr) = a <- (translate (HModSem.wrap scopes) itr);; (translate (HModSem.wrap scopes) (ktr a))
   .
   Proof. rewrite (bisim_is_eq (translate_bind _ _ _)); eauto. Qed.
 
   Lemma transl_tau
     A
-    keys
+    scopes
     (itr: itree hmodE A)
   :
-    translate (HModSem.wrap keys) (tau;; itr) = tau;; (translate (HModSem.wrap keys) itr)
+    translate (HModSem.wrap scopes) (tau;; itr) = tau;; (translate (HModSem.wrap scopes) itr)
   .
   Proof. rewrite (bisim_is_eq (translate_tau _ _)); eauto. Qed.
 
   Lemma transl_ret
-      A (a: A) keys
+      A (a: A) scopes
   :
-    translate (HModSem.wrap keys) (Ret a) = Ret a
+    translate (HModSem.wrap scopes) (Ret a) = Ret a
   .
   Proof. rewrite (bisim_is_eq (translate_ret _ _)); eauto. Qed.
 
   Lemma transl_call
-    keys fn args
+    scopes fn args
   :
-  translate (HModSem.wrap keys) (trigger (Call fn args)) = trigger (Call fn args)
+  translate (HModSem.wrap scopes) (trigger (Call fn args)) = trigger (Call fn args)
   .
   Proof.
     unfold trigger. rewrite (bisim_is_eq (translate_vis _ _ _ _)). ss.
@@ -178,41 +156,43 @@ Section RED.
   Qed.
 
   Lemma transl_put
-    keys k v
+    scopes k v
   :
-  translate (HModSem.wrap keys) (trigger (SPut k v)) =
-    if existsb (eqb k) keys then trigger (SPut k v) else trigger (Choose Any.t)
+  translate (HModSem.wrap scopes) (trigger (SPut k v)) =
+    if existsb (eqb k.1) scopes then trigger (SPut k v) else trigger (Choose Any.t)
   .
   Proof.
-    unfold trigger. rewrite (bisim_is_eq (translate_vis _ _ _ _)). ss.
-    des_ifs; s; do 2 f_equal; extensionalities; rewrite transl_ret; eauto.
+    unfold trigger. destruct k. s.
+    rewrite (bisim_is_eq (translate_vis _ _ _ _)). ss.
+    des_ifs; s; do 2 f_equal; extensionalities; try rewrite transl_ret; eauto.
   Qed.
 
   Lemma transl_get
-    keys k
+    scopes k
   :
-  translate (HModSem.wrap keys) (trigger (SGet k)) =
-    if existsb (eqb k) keys then trigger (SGet k) else trigger (Choose Any.t)
+  translate (HModSem.wrap scopes) (trigger (SGet k)) =
+    if existsb (eqb k.1) scopes then trigger (SGet k) else trigger (Choose Any.t)
   .
   Proof.
-    unfold trigger. rewrite (bisim_is_eq (translate_vis _ _ _ _)). ss.
+    unfold trigger. destruct k. s.
+    rewrite (bisim_is_eq (translate_vis _ _ _ _)). ss.
     des_ifs; s; do 2 f_equal; extensionalities; rewrite transl_ret; eauto.
   Qed.
   
   Lemma transl_core
-    T keys
+    T scopes
     (e: coreE T)
     :
-    translate (HModSem.wrap keys) (trigger e) = trigger e.
+    translate (HModSem.wrap scopes) (trigger e) = trigger e.
   Proof.
     unfold trigger. rewrite (bisim_is_eq (translate_vis _ _ _ _)). ss.
     des_ifs; s; do 2 f_equal; extensionalities; rewrite transl_ret; eauto.
   Qed.
 
   Lemma transl_Assume
-    keys P
+    scopes P
   :
-    translate (HModSem.wrap keys) (trigger (Assume P)) = trigger (Assume P)
+    translate (HModSem.wrap scopes) (trigger (Assume P)) = trigger (Assume P)
   .
   Proof.
     unfold trigger.
@@ -222,9 +202,9 @@ Section RED.
   Qed.
 
   Lemma transl_Guarantee
-    keys P
+    scopes P
   :
-    translate (HModSem.wrap keys) (trigger (Guarantee P)) = trigger (Guarantee P)
+    translate (HModSem.wrap scopes) (trigger (Guarantee P)) = trigger (Guarantee P)
   .
   Proof.
     unfold trigger.
@@ -235,9 +215,9 @@ Section RED.
   
 (*  
   Lemma transl_triggerUB
-    T keys
+    T scopes
   :
-    translate (HModSem.wrap keys) (triggerUB: itree _ T) = triggerUB
+    translate (HModSem.wrap scopes) (triggerUB: itree _ T) = triggerUB
   .
   Proof.
     unfold triggerUB. rewrite transl_bind. f_equal.
@@ -246,9 +226,9 @@ Section RED.
   Qed.
 
   Lemma transl_triggerNB
-    T keys
+    T scopes
   :
-    translate (HModSem.wrap keys) (triggerNB: itree _ T) = triggerNB
+    translate (HModSem.wrap scopes) (triggerNB: itree _ T) = triggerNB
   .
   Proof.
     unfold triggerNB. rewrite transl_bind. f_equal.
@@ -257,9 +237,9 @@ Section RED.
   Qed.
 
   Lemma transl_unwrapU
-    R keys (r: option R)
+    R scopes (r: option R)
   :
-    translate (HModSem.wrap keys) (unwrapU r) = unwrapU r
+    translate (HModSem.wrap scopes) (unwrapU r) = unwrapU r
   .
   Proof.
     unfold unwrapU. destruct r.
@@ -268,9 +248,9 @@ Section RED.
   Qed.
 
   Lemma transl_unwrapN
-    R keys (r: option R)
+    R scopes (r: option R)
   :
-    translate (HModSem.wrap keys) (unwrapN r) = unwrapN r
+    translate (HModSem.wrap scopes) (unwrapN r) = unwrapN r
   .
   Proof.
     unfold unwrapN. destruct r.
@@ -279,9 +259,9 @@ Section RED.
   Qed.
 
   Lemma transl_asm
-    keys P
+    scopes P
   :
-    translate (HModSem.wrap keys) (assume P) = assume P
+    translate (HModSem.wrap scopes) (assume P) = assume P
   .
   Proof.
     unfold assume, trigger.
@@ -293,9 +273,9 @@ Section RED.
   Qed.
 
   Lemma transl_guar
-    keys P
+    scopes P
   :
-    translate (HModSem.wrap keys) (guarantee P) = guarantee P
+    translate (HModSem.wrap scopes) (guarantee P) = guarantee P
   .
   Proof.
     unfold guarantee, trigger.
@@ -307,10 +287,10 @@ Section RED.
   Qed.
 
   Lemma transl_ext
-    T keys (itr0 itr1: itree _ T)
+    T scopes (itr0 itr1: itree _ T)
     (EQ: itr0 = itr1)
   :
-    translate (HModSem.wrap keys) itr0 = translate (HModSem.wrap keys) itr1
+    translate (HModSem.wrap scopes) itr0 = translate (HModSem.wrap scopes) itr1
   .
   Proof. subst. refl. Qed.
  *)
