simulations/ctxrefine/CtxRefine.v
@@ -24,15 +24,16 @@ Section CTX_REFINE.
   Context `{Sk.ld}.
 
   Definition refines (md_src md_tgt: HMod.t): Prop :=
-    let Ps := HModSem.initial_cond (md_src.(HMod.get_modsem) md_src.(HMod.sk)) in
-    let Pt := HModSem.initial_cond (md_tgt.(HMod.get_modsem) md_tgt.(HMod.sk)) in
-    (forall rs (SRC: Ps rs), exists rt (TGT: Pt rt),
-    refines_mod (HMod.to_mod md_src rs) (HMod.to_mod md_tgt rt)).
+    let Ps := md_src.(HMod.get_modsem) md_src.(HMod.sk) in
+    let Pt := md_tgt.(HMod.get_modsem) md_tgt.(HMod.sk) in
+
+    forall rs (WF: Ps.(HModSem.wf)) (SRC: Ps.(HModSem.initial_cond) rs),
+    exists rt, Pt.(HModSem.wf) /\ Pt.(HModSem.initial_cond) rt /\
+    refines_mod (HMod.to_mod md_src rs) (HMod.to_mod md_tgt rt).
 
   Definition ctx_refines (md_src md_tgt: HMod.t): Prop :=
     forall (ctx: HMod.t),
-      refines (HMod.add md_src ctx) (HMod.add md_tgt ctx).
-
+    refines (HMod.add md_src ctx) (HMod.add md_tgt ctx).
 
   (* To be moved *)
   
